PAC: more

PAC/PAC_Checker_Specification.thy
@@ -5,6 +5,16 @@ theory PAC_Checker_Specification
 
 begin
 
+
+datatype 'a status =
+  is_failed: FAILED (status_error: 'a) |
+  is_success: SUCCESS |
+  is_found: FOUND
+
+lemma is_success_alt_def:
+  \<open>is_success a \<longleftrightarrow> a = SUCCESS\<close>
+  by (cases a) auto
+
 datatype 'a pac_step =
   AddD (pac_src1: nat) (pac_src2: nat) (new_id: nat) (pac_res: 'a) |
   Add (pac_src1: nat) (pac_src2: nat) (new_id: nat) (pac_res: 'a) |
@@ -12,14 +22,24 @@ datatype 'a pac_step =
   Mult (pac_src1: nat) (pac_mult: 'a) (new_id: nat) (pac_res: 'a)
 
 
-definition PAC_checker_specification ::  \<open>int_poly multiset \<Rightarrow> (bool \<times> int_poly multiset) nres\<close> where
-  \<open>PAC_checker_specification A = SPEC(\<lambda>(b, B). b \<longrightarrow> ideal (set_mset B) \<subseteq> ideal (set_mset A))\<close>
+definition PAC_checker_specification
+  :: \<open>int_poly multiset \<Rightarrow> int_poly \<Rightarrow> ('a status \<times> int_poly multiset) nres\<close>
+where
+  \<open>PAC_checker_specification A spec = SPEC(\<lambda>(b, B).
+      (\<not>is_failed b \<longrightarrow> ideal (set_mset B) \<subseteq> ideal (set_mset A)) \<and>
+      (is_found b \<longrightarrow> spec \<in> ideal (set_mset A)))\<close>
 
-definition PAC_checker_specification_spec ::  \<open>int_poly multiset \<Rightarrow> (bool \<times> int_poly multiset) \<Rightarrow> bool\<close> where
-  \<open>PAC_checker_specification_spec A = (\<lambda>(b, B). b \<longrightarrow> PAC_Format\<^sup>*\<^sup>* (A) (B))\<close>
+definition PAC_checker_specification_spec
+  ::  \<open>int_poly \<Rightarrow> int_poly multiset \<Rightarrow> ('a status \<times> int_poly multiset) \<Rightarrow> bool\<close>
+where
+  \<open>PAC_checker_specification_spec spec A = (\<lambda>(b, B).
+       (is_success b \<longrightarrow> PAC_Format\<^sup>*\<^sup>* A B) \<and>
+       (is_found b \<longrightarrow> PAC_Format\<^sup>*\<^sup>* A B \<and> spec \<in> pac_ideal (set_mset A)))\<close>
 
-abbreviation PAC_checker_specification2 ::  \<open>int_poly multiset \<Rightarrow> (bool \<times> int_poly multiset) nres\<close> where
-  \<open>PAC_checker_specification2 A \<equiv> SPEC(PAC_checker_specification_spec A)\<close>
+abbreviation PAC_checker_specification2
+  ::  \<open>int_poly \<Rightarrow> int_poly multiset \<Rightarrow> ('a status \<times> int_poly multiset) nres\<close>
+where
+  \<open>PAC_checker_specification2 spec A \<equiv> SPEC(PAC_checker_specification_spec spec A)\<close>
 
 definition normalize_poly_spec :: \<open>_\<close> where
   \<open>normalize_poly_spec p = SPEC (\<lambda>r. p - r \<in> ideal polynom_bool)\<close>
@@ -42,48 +62,61 @@ definition check_mult :: \<open>(nat, int mpoly) fmap \<Rightarrow> nat \<Righta
      SPEC(\<lambda>b. b \<longrightarrow> p \<in># dom_m A \<and>i \<notin># dom_m A \<and>
             the (fmlookup A p) * q - r \<in>  ideal polynom_bool)\<close>
 
+fun merge_status where
+  \<open>merge_status (FAILED a) _ = FAILED a\<close> |
+  \<open>merge_status _ (FAILED a) = FAILED a\<close> |
+  \<open>merge_status FOUND _ = FOUND\<close> |
+  \<open>merge_status _ FOUND = FOUND\<close> |
+  \<open>merge_status _ _ = SUCCESS\<close>
 
-definition PAC_checker_step ::  \<open>(nat, int_poly) fmap  \<Rightarrow> int_poly pac_step \<Rightarrow> (bool \<times> (nat, int_poly) fmap) nres\<close> where
-  \<open>PAC_checker_step A st = (case st of
+definition PAC_checker_step
+  ::  \<open>int_poly \<Rightarrow> unit status \<times> (nat, int_poly) fmap \<Rightarrow> int_poly pac_step \<Rightarrow>
+    (unit status \<times> (nat, int_poly) fmap) nres\<close>
+where
+  \<open>PAC_checker_step = (\<lambda>spec (stat, A) st. case st of
      AddD _ _ _ _ \<Rightarrow>
        do {
         r \<leftarrow> normalize_poly_spec (pac_res st);
         eq \<leftarrow> check_add A (pac_src1 st) (pac_src2 st) (new_id st) r;
+        st' \<leftarrow> SPEC(\<lambda>st'. \<not>is_failed st' \<and> (is_found st' \<longrightarrow> r - spec \<in> ideal polynom_bool));
         if eq
-        then RETURN (True,
+        then RETURN (merge_status stat st',
           fmupd (new_id st) r
             (fmdrop (pac_src1 st) (fmdrop (pac_src2 st) A)))
-        else RETURN (False, A)
+        else RETURN (FAILED (), A)
    }
    | Add _ _ _ _ \<Rightarrow>
        do {
          r \<leftarrow> normalize_poly_spec (pac_res st);
         eq \<leftarrow> check_add A (pac_src1 st) (pac_src2 st) (new_id st) r;
+        st' \<leftarrow> SPEC(\<lambda>st'. is_success st' \<or> (is_found st' \<longrightarrow> r - spec \<in> ideal polynom_bool));
         if eq
-        then RETURN (True,
+        then RETURN (merge_status stat st',
           fmupd (new_id st) r A)
-        else RETURN (False, A)
+        else RETURN (FAILED (), A)
    }
    | MultD _ _ _ _ \<Rightarrow>
        do {
          r \<leftarrow> normalize_poly_spec (pac_res st);
          q \<leftarrow> normalize_poly_spec (pac_mult st);
         eq \<leftarrow> check_mult A (pac_src1 st) q (new_id st) r;
+        st' \<leftarrow> SPEC(\<lambda>st'. is_success st' \<or> (is_found st' \<longrightarrow> r - spec \<in> ideal polynom_bool));
         if eq
-        then RETURN (True,
+        then RETURN (merge_status stat st',
           fmupd (new_id st) r
             (fmdrop (pac_src1 st) A))
-        else RETURN (False, A)
+        else RETURN (FAILED (), A)
    }
    | Mult _ _ _ _ \<Rightarrow>
        do {
          r \<leftarrow> normalize_poly_spec (pac_res st);
          q \<leftarrow> normalize_poly_spec (pac_mult st);
         eq \<leftarrow> check_mult A (pac_src1 st) q (new_id st) r;
+        st' \<leftarrow> SPEC(\<lambda>st'. is_success st' \<or> (is_found st' \<longrightarrow> r - spec \<in> ideal polynom_bool));
         if eq
-        then RETURN (True,
+        then RETURN (merge_status stat st',
           fmupd (new_id st) r A)
-        else RETURN (False, A)
+        else RETURN (FAILED (), A)
    }
  )\<close>
 
@@ -184,10 +217,110 @@ lemma PAC_Format_add_and_remove:
     done
   done
 
+
+definition status_rel where
+  \<open>status_rel = {(SUCCESS, SUCCESS), (FOUND, FOUND)} \<union>
+    (\<lambda>(a, b). (FAILED a, FAILED b)) ` (UNIV \<times> UNIV)\<close>
+
+lemma status_rel_intro[iff,simp]:
+  \<open>(FAILED a, FAILED b) \<in> status_rel\<close>
+  \<open>(SUCCESS,SUCCESS) \<in> status_rel\<close>
+  \<open>(FOUND,FOUND) \<in> status_rel\<close>
+  \<open>(FAILED a, SUCCESS) \<notin> status_rel\<close>
+  \<open>(FAILED a, FOUND) \<notin> status_rel\<close>
+  \<open>(SUCCESS,FAILED a) \<notin> status_rel\<close>
+  \<open>(SUCCESS,FOUND) \<notin> status_rel\<close>
+  \<open>(FOUND,SUCCESS) \<notin> status_rel\<close>
+  \<open>(FOUND,FAILED a) \<notin> status_rel\<close>
+  by (auto simp: status_rel_def)
+
+lemma status_rel_alt_def:
+  \<open>(a, b) \<in> status_rel \<longleftrightarrow>
+     (is_failed a = is_failed b) \<and>
+     (is_success a = is_success b) \<and>
+     (is_found a = is_found b)\<close>
+   by (cases a; cases b) auto
+
+lemma is_merge_status[simp]:
+  \<open>is_failed (merge_status a st') \<longleftrightarrow> is_failed a \<or> is_failed st'\<close>
+  \<open>is_found (merge_status a st') \<longleftrightarrow> \<not>is_failed a \<and> \<not>is_failed st' \<and> (is_found a \<or> is_found st')\<close>
+  \<open>is_success (merge_status a st') \<longleftrightarrow> (is_success a \<and> is_success st')\<close>
+  by (cases a; cases st'; auto; fail)+
+
+lemma status_rel_merge_status:
+  \<open>(merge_status a b, SUCCESS) \<notin> status_rel \<longleftrightarrow>
+    (\<exists>a'. a = FAILED a') \<or> (\<exists>a'. b = FAILED a') \<or>
+    a = FOUND \<or> (b = FOUND)\<close>
+  by (cases a; cases b; auto)
+
+lemma Ex_status_iff:
+  \<open>(\<exists>a. P a) \<longleftrightarrow> P SUCCESS \<or> P FOUND \<or> (\<exists>a. P (FAILED a))\<close>
+  apply auto
+  apply (case_tac a; auto)
+  done
+
+lemma is_failed_alt_def:
+  \<open>is_failed st' \<longleftrightarrow> \<not>is_success st' \<and> \<not>is_found st'\<close>
+  by (cases st') auto
+
+lemma merge_status_eq_iff[simp]:
+  \<open>merge_status a SUCCESS = SUCCESS \<longleftrightarrow> a = SUCCESS\<close>
+  \<open>merge_status a SUCCESS = FOUND \<longleftrightarrow> a = FOUND\<close>
+  \<open>merge_status SUCCESS a = SUCCESS \<longleftrightarrow> a = SUCCESS\<close>
+  \<open>merge_status SUCCESS a = FOUND \<longleftrightarrow> a = FOUND\<close>
+  \<open>merge_status SUCCESS a = FAILED b \<longleftrightarrow> a = FAILED b\<close>
+  \<open>merge_status a SUCCESS = FAILED b \<longleftrightarrow> a = FAILED b\<close>
+  \<open>merge_status FOUND a = FAILED b \<longleftrightarrow> a = FAILED b\<close>
+  \<open>merge_status a FOUND = FAILED b \<longleftrightarrow> a = FAILED b\<close>
+  \<open>merge_status a FOUND = SUCCESS \<longleftrightarrow> False\<close>
+  by (cases a; auto; fail)+
+
+find_theorems "is_success _ \<longleftrightarrow> _"
 lemma PAC_checker_step_PAC_checker_specification2:
-  assumes \<open>(A,B) \<in> polys_rel\<close>
-  shows \<open>PAC_checker_step A st \<le> \<Down> (bool_rel \<times>\<^sub>r polys_rel) (PAC_checker_specification2 B)\<close>
+  fixes a :: \<open>unit status\<close>
+  assumes [simp,intro]: \<open>(A,B) \<in> polys_rel\<close> and
+    \<open>\<not>is_failed a\<close> and
+    [simp,intro]: \<open>a = FOUND \<Longrightarrow> spec \<in> pac_ideal (set_mset B)\<close>
+  shows \<open>PAC_checker_step spec (a, A) st \<le> \<Down> (status_rel \<times>\<^sub>r polys_rel) (PAC_checker_specification2 spec B)\<close>
 proof -
+  have H1: \<open> x12 \<in># dom_m A \<Longrightarrow>
+       2 * the (fmlookup A x12) - r \<in> More_Modules.ideal polynom_bool \<Longrightarrow>
+       r - spec \<in> More_Modules.ideal polynom_bool \<Longrightarrow>
+       spec \<in> pac_ideal (set_mset B)\<close> for x12 r
+     using \<open>(A,B) \<in> polys_rel\<close>
+      ideal.span_add[OF ideal.span_add[OF ideal.span_neg ideal.span_neg,
+         of \<open>the (fmlookup A x12)\<close> _  \<open>the (fmlookup A x12)\<close>],
+      of \<open>set_mset B \<union> polynom_bool\<close> \<open>2 * the (fmlookup A x12) - r\<close>]
+     unfolding polys_rel_def
+    apply (subgoal_tac \<open>r \<in> pac_ideal (set_mset B)\<close>)
+     apply (auto dest!: multi_member_split simp: ran_m_def)
+     apply (metis Un_insert_left diff_in_polynom_bool_pac_idealI ideal.span_diff ideal.span_zero)
+     by (metis (no_types, lifting) UnCI Un_insert_left diff_in_polynom_bool_pac_idealI ideal.span_add ideal.span_base mult_2 set_image_mset set_mset_add_mset_insert union_single_eq_member)
+
+  have H2: \<open>x11 \<in># dom_m A \<Longrightarrow>
+       x12 \<in># dom_m A \<Longrightarrow>
+       the (fmlookup A x11) + the (fmlookup A x12) - r
+       \<in> More_Modules.ideal polynom_bool \<Longrightarrow>
+       r - spec \<in> More_Modules.ideal polynom_bool \<Longrightarrow>
+       spec \<in> pac_ideal (set_mset B)\<close>  for x12 r x11
+     using \<open>(A,B) \<in> polys_rel\<close>
+      ideal.span_add[OF ideal.span_add[OF ideal.span_neg ideal.span_neg,
+         of \<open>the (fmlookup A x11)\<close> _  \<open>the (fmlookup A x12)\<close>],
+      of \<open>set_mset B \<union> polynom_bool\<close> \<open>the (fmlookup A x11) + the (fmlookup A x12) - r\<close>]
+     unfolding polys_rel_def
+    apply (subgoal_tac \<open>r \<in> pac_ideal (set_mset B)\<close>)
+     apply (auto dest!: multi_member_split simp: ran_m_def ideal.span_base)
+     apply (metis Un_insert_left diff_in_polynom_bool_pac_idealI ideal.span_diff ideal.span_zero)
+     by (smt Un_insert_left diff_diff_eq2 diff_in_polynom_bool_pac_idealI diff_zero ideal.span_base ideal.span_diff ideal.span_neg insertI1 minus_diff_eq)
+
+  have eq_successI: \<open>st' \<noteq> FAILED () \<Longrightarrow>
+       st' \<noteq> FOUND \<Longrightarrow> st' = SUCCESS\<close> for st'
+    by (cases st') auto
+  have [iff]: \<open>a \<noteq> FAILED ()\<close> and
+    [intro]: \<open>a \<noteq> SUCCESS \<Longrightarrow> a = FOUND\<close> and
+    [simp]: \<open>merge_status a FOUND = FOUND\<close>
+    using assms(2) by (cases a; auto)+
+  note [[goals_limit=1]]
   show ?thesis
     unfolding PAC_checker_step_def PAC_checker_specification_spec_def
       normalize_poly_spec_alt_def check_mult_def check_add_def
@@ -199,13 +332,25 @@ proof -
       apply (auto 6 4 simp: RETURN_def 
         intro: PAC_Format.intros simp flip: insert_minus_eq)
       apply (rule RES_refine)
-      apply auto
-      defer
+      apply (auto simp: Ex_status_iff)
       apply (rule RES_refine)
-      apply auto
+      apply (auto simp: Ex_status_iff)
       apply (rule RES_refine)
-      apply (rule_tac x = \<open>(True, add_mset r B - (if x11 \<noteq> x12 then {#the (fmlookup A x11), the (fmlookup A x12)#} else {#the (fmlookup A x11)#}))\<close> in bexI)
-      apply (auto simp: polys_rel_update_remove PAC_Format_add_and_remove)
+      apply (rule_tac x = \<open>(if a = SUCCESS then SUCCESS else FOUND,add_mset r B - (if x11 \<noteq> x12 then {#the (fmlookup A x11), the (fmlookup A x12)#} else {#the (fmlookup A x11)#}))\<close> in bexI)
+      apply (auto simp: polys_rel_update_remove PAC_Format_add_and_remove
+           status_rel_alt_def is_failed_def is_success_def is_found_def
+        dest!: eq_successI
+        split: if_splits)[2]
+      apply (rule RES_refine)
+      apply (auto simp: status_rel_alt_def Ex_status_iff)
+      apply (rule RES_refine)
+      apply (rule_tac x = \<open>(if a = FOUND \<or> st' = FOUND then FOUND else SUCCESS,add_mset r B - (if x11 \<noteq> x12 then {#the (fmlookup A x11), the (fmlookup A x12)#} else {#the (fmlookup A x11)#}))\<close> in bexI)
+      apply (auto simp: polys_rel_update_remove PAC_Format_add_and_remove
+           status_rel_alt_def is_failed_def is_success_def is_found_def H1 H2
+        dest!: eq_successI
+        split: if_splits)[2]
+      apply (rule RES_refine)
+      apply (auto simp: status_rel_alt_def Ex_status_iff)
       done
     subgoal
       apply refine_vcg
@@ -253,41 +398,46 @@ proof -
 qed
 
 
-definition PAC_checker:: \<open>(nat, int_poly) fmap \<Rightarrow> int_poly pac_step list \<Rightarrow> (bool \<times> (nat, int_poly) fmap) nres\<close> where
-  \<open>PAC_checker A st = do {
+definition PAC_checker
+  :: \<open>int_poly \<Rightarrow> (nat, int_poly) fmap \<Rightarrow> int_poly pac_step list \<Rightarrow>
+    (unit status \<times> (nat, int_poly) fmap) nres\<close>
+where
+  \<open>PAC_checker spec A st = do {
     (S, _) \<leftarrow> WHILE\<^sub>T
-       (\<lambda>((b, A), n::nat). b \<and> n < length st)
-       (\<lambda>((b, A), n). do {
+       (\<lambda>((b :: unit status, A :: (nat, int_poly) fmap), n::nat). \<not>is_failed b \<and> n < length st)
+       (\<lambda>((bA), n). do {
           ASSERT(n < length st);
-          S \<leftarrow> PAC_checker_step A (st ! n);
+          S \<leftarrow> PAC_checker_step spec (bA) (st ! n);
           RETURN (S, (n+1))
         })
-      ((True, A), 0);
+      ((SUCCESS, A), 0);
     RETURN S
   }\<close>
 
 
 lemma PAC_checker_specification_spec_trans:
-  \<open>PAC_checker_specification_spec A (True, x2) \<Longrightarrow>
-    PAC_checker_specification_spec x2 x1a \<Longrightarrow>
-    PAC_checker_specification_spec A x1a\<close>
+  \<open>PAC_checker_specification_spec spec A (st, x2) \<Longrightarrow>
+    PAC_checker_specification_spec spec x2 (st, x1a) \<Longrightarrow>
+    PAC_checker_specification_spec spec A (st, x1a)\<close>
  unfolding PAC_checker_specification_spec_def
  by auto
 
 lemma RES_SPEC_eq:
   \<open>RES \<Phi> = SPEC(\<lambda>P. P \<in> \<Phi>)\<close>
   by auto
+
 lemma PAC_checker_PAC_checker_specification2:
-  \<open>(A, B) \<in> polys_rel \<Longrightarrow> PAC_checker A st \<le> \<Down> (bool_rel \<times>\<^sub>r polys_rel) (PAC_checker_specification2 B)\<close>
+  \<open>(A, B) \<in> polys_rel \<Longrightarrow>
+  PAC_checker spec A st \<le> \<Down> (status_rel \<times>\<^sub>r polys_rel) (PAC_checker_specification2 spec B)\<close>
   unfolding PAC_checker_def conc_fun_RES
   apply (subst RES_SPEC_eq)
   apply (refine_vcg WHILET_rule[where
-      I = \<open>\<lambda>((bB), n). n \<le> length st \<and> bB \<in> (bool_rel \<times>\<^sub>r polys_rel)\<inverse> ``
-                      Collect (PAC_checker_specification_spec B)\<close>
+      I = \<open>\<lambda>((bB), n). n \<le> length st \<and> bB \<in> (status_rel \<times>\<^sub>r polys_rel)\<inverse> ``
+                      Collect (PAC_checker_specification_spec spec B)\<close>
     and R = \<open>measure (\<lambda>(_, n).  Suc (length st) - n)\<close>])
   subgoal by auto
   subgoal by auto
-  subgoal by (force simp: PAC_checker_specification_spec_def)
+  subgoal by (force simp: PAC_checker_specification_spec_def status_rel_def)
   subgoal by auto
   subgoal
     apply auto
